obtain_invariant_3

concurrency/scache/CacheSpec.s.dfy
@@ -1,5 +1,6 @@
 include "../framework/StateMachines.s.dfy"
 include "../../lib/Lang/NativeTypes.s.dfy"
+include "../framework/DiskSSM.s.dfy"
 
 module CacheIfc refines InputOutputIfc {
   import opened NativeTypes
@@ -17,6 +18,8 @@ module CacheIfc refines InputOutputIfc {
 
 module CacheSpec refines StateMachine(CrashAsyncIfc(CacheIfc)) {
   import opened NativeTypes
+  import opened RequestIds
+  import CacheIfc
 
   type Value = seq<byte>
 
@@ -28,74 +31,83 @@ module CacheSpec refines StateMachine(CrashAsyncIfc(CacheIfc)) {
   datatype Variables = Variables(
     store: map<int, VersionedObject>,
 
-    reqs: map<RequestId, IOIfc.Input>,
-    resps: map<RequestId, IOIfc.Output>,
+    reqs: map<RequestId, CacheIfc.Input>,
+    resps: map<RequestId, CacheIfc.Output>,
 
     // RequestId -> key -> version
     // means that for the RequestId to complete, the 'persistence'
     // at key 'key' must be >= version
-    syncReqs: map<RequestId, map<int, int>>
+    syncs: map<RequestId, map<int, int>>
   )
 
-  predicate PushInput(s: Variables, s': Variable, op: ifc.Op,
+  predicate PushInput(s: Variables, s': Variables, op: ifc.Op,
         rid: RequestId, input: CacheIfc.Input)
   {
-    && op == Start(rid, input)
+    && op == ifc.Start(rid, input)
     && (input.WriteInput? || input.ReadInput?)
     && rid !in s.reqs
     && s' == s.(reqs := s.reqs[rid := input])
   }
 
-  predicate Process(s: Variables, s': Variable, op: ifc.Op,
+  predicate Process(s: Variables, s': Variables, op: ifc.Op,
         rid: RequestId)
   {
-    && op == InternalOp
+    && op == ifc.InternalOp
     && rid in s.reqs
     && (s.reqs[rid].WriteInput? ==>
-      s.(store := s.store[s.reqs[rid].key := s.reqs[rid].data])
-      s.(reqs := s.reqs - {rid})
-      s.(resps := s.resps[rid := WriteOutput])
+      s' ==
+        s.(store := s.store[s.reqs[rid].key :=
+            VersionedObject(
+              s.store[s.reqs[rid].key].versions + [s.reqs[rid].data],
+              s.store[s.reqs[rid].key].persistent)])
+         .(reqs := s.reqs - {rid})
+         .(resps := s.resps[rid := CacheIfc.WriteOutput])
+    )
+    && (s.reqs[rid].ReadInput? ==>
+      s' ==
+        s.(reqs := s.reqs - {rid})
+         .(resps := s.resps[rid := CacheIfc.ReadOutput(
+            s.store[s.reqs[rid].key].versions[
+                |s.store[s.reqs[rid].key].versions| - 1])])
     )
   }
 
-  predicate PopOutput(s: Variables, s': Variable, op: ifc.Op,
-      rid: RequestId, output: CacheIfc.Output)
+  predicate PopOutput(s: Variables, s': Variables, op: ifc.Op, rid: RequestId)
   {
-    && op == End(rid, output)
     && rid in s.resps
+    && op == ifc.End(rid, s.resps[rid])
     && s' == s.(resps := s.resps - {rid})
-    && output == s.resps[rid]
   }
 
   predicate PushSync(s: Variables, s': Variables, op: ifc.Op, rid: RequestId)
   {
-    && op == Start(rid, SyncInput)
-    && rid !in s.syncReqs
-    && s' == s.(syncReqs := s.syncReqs[rid :=
-        (map key | key in s.store :: |s.store[key].versions| - 1))
+    && op == ifc.Start(rid, CacheIfc.SyncInput)
+    && rid !in s.syncs
+    && s' == s.(syncs := s.syncs[rid :=
+        (map key | key in s.store :: |s.store[key].versions| - 1)])
   }
 
   predicate PopSync(s: Variables, s': Variables, op: ifc.Op, rid: RequestId) {
-    && op == End(rid, SyncOutput)
-    && rid in s.syncResps
+    && op == ifc.End(rid, CacheIfc.SyncOutput)
+    && rid in s.syncs
     && s' == s.(resps := s.resps - {rid})
-    && (forall key | key in s.syncReqs[rid]
-            :: key in s.store && s.store[key].persistent >= s.syncReqs[rid][key])
+    && (forall key | key in s.syncs[rid]
+            :: key in s.store && s.store[key].persistent >= s.syncs[rid][key])
   }
 
   predicate VersionedObjectPersist(v: VersionedObject, v': VersionedObject) {
     && v'.versions == v.versions
-    && v.persistent <= v'.persistent < |v.versions|)
+    && v.persistent <= v'.persistent < |v.versions|
   }
 
   predicate Persist(s: Variables, s': Variables, op: ifc.Op) {
-    && op == InternalOp
+    && op == ifc.InternalOp
     && s'.reqs == s.reqs
     && s'.resps == s.resps
-    && s'.syncReqs == s.syncReqs
+    && s'.syncs == s.syncs
     && (forall key :: key in s.store <==> key in s'.store)
     && (forall key :: key in s.store ==> key in s'.store
-        && VersionedObjectPersist(s.store[key], s'.store[key])
+        && VersionedObjectPersist(s.store[key], s'.store[key]))
   }
 
   predicate VersionedObjectCrash(v: VersionedObject, v': VersionedObject, op: ifc.Op) {
@@ -106,13 +118,39 @@ module CacheSpec refines StateMachine(CrashAsyncIfc(CacheIfc)) {
   }
 
   predicate Crash(s: Variables, s': Variables, op: ifc.Op) {
-    && op == CrashOp
+    && op == ifc.CrashOp
     && s'.reqs == map[]
     && s'.resps == map[]
-    && s'.syncReqs == map[]
+    && s'.syncs == map[]
+    && (forall key :: key in s.store <==> key in s'.store)
     && (forall key | key in s.store ::
           && key in s'.store
           && VersionedObjectCrash(s.store[key], s'.store[key])
        )
+  }
+
+  datatype Step =
+    | PushInputStep(rid: RequestId, input: CacheIfc.Input)
+    | ProcessStep(rid: RequestId)
+    | PopOutputStep(rid: RequestId)
+    | PushSyncStep(rid: RequestId)
+    | PopSyncStep(rid: RequestId)
+    | PersistStep
+    | CrashStep
+
+  predicate NextStep(s: Variables, s': Variables, op: ifc.Op, step: Step) {
+    match step {
+      case PushInputStep(rid, input) => PushInput(s, s', op, rid, input)
+      case ProcessStep(rid) => Process(s, s', op, rid)
+      case PopOutputStep(rid) => PopOutput(s, s', op, rid)
+      case PushSyncStep(rid) => PushSync(s, s', op, rid)
+      case PopSyncStep(rid) => PopSync(s, s', op, rid)
+      case PersistStep => Persist(s, s', op)
+      case CrashStep => Persist(s, s', op)
+    }
+  }
+
+  predicate Next(s: Variables, s': Variables, op: ifc.Op) {
+    exists step :: NextStep(s, s', op, step)
   }
 }
